refine FormOptSolver.v

FormOptSolver.v
@@ -1,214 +1,126 @@
-Require Import Formula Find.
-
+Require Import Formula FindVal.
+Require Import Btauto.
 
 
 Fixpoint formula_optimizer (p : form): form :=
   match p with
   | var _ => p
-  | bool _  => p
-  | land (var x) (bool true) => (var x)
-  | land (var x) (bool false) => (bool false)
-  | land (bool true) (var x) => (var x) 
-  | land (bool false) (var x) => (bool false)                                
+  | boolv _  => p
+  | land (var x) (boolv true) => (var x)
+  | land (var x) (boolv false) => (boolv false)
+  | land (boolv true) (var x) => (var x) 
+  | land (boolv false) (var x) => (boolv false)                                
   | land p1 p2 => land (formula_optimizer p1) (formula_optimizer p2)
-  | lor (var x) (bool true) => (bool true)
-  | lor (var x) (bool false) => (var x) 
-  | lor (bool true) (var x) => (bool true)
-  | lor (bool false) (var x) => (var x) 
+  | lor (var x) (boolv true) => (boolv true)
+  | lor (var x) (boolv false) => (var x) 
+  | lor (boolv true) (var x) => (boolv true)
+  | lor (boolv false) (var x) => (var x) 
   | lor p1 p2 => lor (formula_optimizer p1) (formula_optimizer p2)
   | mapsto p1 p2 => mapsto (formula_optimizer p1) (formula_optimizer p2)
   | not p => not (formula_optimizer p)
   end.
 
 
-Lemma land_interp : forall (V : valuation) (p1 p2 : form),interp V  (land p1 p2) = interp V  p1 && interp V p2.
-Proof.
-  intros.
-  destruct p1,p2;(try unfold interp;reflexivity).
-  Qed.
   
-  
-Lemma opt_land : forall (V : valuation) (p1 p2 : form),interp V (formula_optimizer (land p1 p2)) = interp V (formula_optimizer p1) && interp V (formula_optimizer p2).
+Lemma interp_opt_land : forall (V : valuation) (p1 p2 : form),interp V (formula_optimizer (land p1 p2)) = interp V (formula_optimizer p1) && interp V (formula_optimizer p2).
   Proof.
     intros.
-    destruct p1 eqn:P1 , p2 eqn:P2;(try unfold formula_optimizer; try apply land_interp);(try destruct b;unfold interp);try (symmetry;apply andb_true_r);try (symmetry;apply andb_true_l);(try symmetry;apply andb_false_r);(try symmetry;apply andb_false_l).
-  Qed.
+    destruct p1 eqn:P1 , p2 eqn:P2;
+      unfold formula_optimizer;
+      try reflexivity; (*trivial cases, form is not changed*)
+      try (destruct b; (*boolv case*)
+       unfold interp).
+      try (btauto). (*land and lor cases*)
+    Qed.
+(**      
+      try (symmetry;apply andb_true_l);
+      try (symmetry;apply andb_false_r);
+      try (symmetry;apply andb_false_l).
+*)
 
 
-Lemma lor_interp : forall (V : valuation) (p1 p2 : form),interp V  (lor p1 p2) = interp V  p1 || interp V p2.
+
+  
+Lemma interp_opt_lor : forall (V : valuation) (p1 p2 : form),interp V (formula_optimizer (lor p1 p2)) = interp V (formula_optimizer p1) || interp V (formula_optimizer p2).
 Proof.
-  intros.
-  destruct p1,p2;(try unfold interp;reflexivity).
-  Qed.
-  
-  
-Lemma opt_lor : forall (V : valuation) (p1 p2 : form),interp V (formula_optimizer (lor p1 p2)) = interp V (formula_optimizer p1) || interp V (formula_optimizer p2).
-  Proof.
     intros.
-    destruct p1 eqn:P1 , p2 eqn:P2;(try unfold formula_optimizer; try apply lor_interp);(try destruct b;unfold interp);try (symmetry;apply orb_true_r); try (symmetry;apply orb_true_l); try (symmetry;apply orb_false_l). try (symmetry;apply orb_false_r).
-Qed.
+    destruct p1 eqn:P1 , p2 eqn:P2;
+      unfold formula_optimizer;
+      try reflexivity; (*trivial cases, form is not changed*)
+      try (destruct b; (*boolv case*)
+           unfold interp);
+      try (btauto). (*land and lor cases*)
+  Qed.
+(**     
+        try (symmetry;apply orb_true_r);
+        try (symmetry;apply orb_true_l);
+        try (symmetry;apply orb_false_l).
+        try (symmetry;apply orb_false_r).
+*)
 
       
 Lemma optimizer_correctness:forall (V : valuation) (p : form), (interp V p) =  (interp V (formula_optimizer p)).
-
 Proof.
   intros.
-  
-  induction p;try reflexivity.
-  - destruct p1  eqn:P1, p2  eqn:P2;(try reflexivity);rewrite  land_interp;rewrite opt_land;try(unfold formula_optimizer; reflexivity);try(rewrite IHp1; rewrite IHp2;reflexivity).
-  - destruct p1  eqn:P1, p2  eqn:P2;(try reflexivity);rewrite  lor_interp;rewrite opt_lor;try(unfold formula_optimizer; reflexivity);try(rewrite IHp1; rewrite IHp2;reflexivity).
-  - unfold formula_optimizer. unfold interp.
+  induction p;try reflexivity. 
+  - rewrite interp_opt_land. (*land *)
+    rewrite <-IHp1, <-IHp2.
+    reflexivity.
+  - rewrite interp_opt_lor. (*lor*)
+    rewrite <-IHp1, <-IHp2.
+    reflexivity.
+  - unfold formula_optimizer. (*mapsto, just rewrite*)
+    unfold interp.
     unfold formula_optimizer in IHp1, IHp2.
     unfold interp in IHp1, IHp2.
-    rewrite IHp1.
-    rewrite IHp2.
+    rewrite IHp1, IHp2.
     reflexivity.
-  - unfold formula_optimizer. unfold interp.
-     unfold formula_optimizer in IHp.
-     unfold interp in IHp.
-     rewrite IHp.
-     reflexivity.
+  - unfold formula_optimizer. (*not, just rewrite*)
+    unfold interp.
+    unfold formula_optimizer in IHp.
+    unfold interp in IHp.
+    rewrite IHp.
+    reflexivity.
 Qed.       
 
 
-
-
-
+(** Integration with solver*)
 
 Definition solver (p : form) :Datatypes.bool:=
-  match find_valuation (formula_optimizer p) with
+  match find_valuation (formula_optimizer p) with (*change here*)
   | Some _ => true
   | None => false
   end.
 
 
-
-
-Lemma land_find_interp: forall p1 p2 V, find_valuation (formula_optimizer (land p1 p2))=Some V -> interp V p1=true /\ interp V p2=true.
-Proof.
-  intros.
-  split;
-    unfold find_valuation in H;
-    unfold try_valuation in H;
-    induction (enum_valuation (collect_var (formula_optimizer (land p1 p2)))); (*add optimizer*)
-    try (discriminate H);
-    try (rewrite <-optimizer_correctness in H;
-         destruct (interp a (land p1 p2)) eqn: E1); (*rewrite to the old proof*)
-    try(inversion H;
-        apply land_interp_interp in E1;
-        destruct E1;
-        rewrite <-H1;
-        assumption);
-    try(apply IHl; (*why it works?*)
-        apply H).
-  Qed.
- 
-
-
-
-
-Lemma lor_find_interp: forall p1 p2 V, find_valuation (formula_optimizer  (lor p1 p2))=Some V -> interp V p1=true \/ interp V p2=true.
-Proof.
-  intros.
-  unfold find_valuation, try_valuation in H.
-  induction (enum_valuation (collect_var (formula_optimizer (lor p1 p2)))). (*add optimizer*)
-  - discriminate H.
-  - rewrite <-optimizer_correctness in H.
-    destruct (interp a (lor p1 p2)) eqn: E1.
-    + inversion H.
-      apply lor_interp_interp in E1.
-      rewrite <-H1.
-      assumption.
-    + apply IHl. (*why it works?*)
-      apply H.
-Qed.
-
-
-
-
-Lemma mapsto_find_interp: forall p1 p2 V, find_valuation (formula_optimizer (mapsto p1 p2))=Some V -> interp V p1=false \/ interp V p2=true.
-Proof.
-  intros.
-  unfold find_valuation,try_valuation in H.
-  induction (enum_valuation (collect_var (formula_optimizer (mapsto p1 p2)))).
-    - discriminate H.
-    - rewrite <-optimizer_correctness in H.
-      destruct (interp a (mapsto p1 p2)) eqn: E1.    
-       + inversion H.
-         apply mapsto_interp_interp in E1.
-         rewrite <-H1.
-         assumption.
-       + apply IHl. (*why it works?*)
-         apply H.
-Qed.
-
-
-
-Lemma not_find_interp: forall p V, find_valuation (formula_optimizer(not p))=Some V -> interp V p=false.
-Proof.
-  intros.
-  unfold find_valuation, try_valuation in H.
-  induction (enum_valuation (collect_var (formula_optimizer (not p)))).
-  - discriminate H.
-  - rewrite <-optimizer_correctness in H.
-    destruct (interp a (not p)) eqn: E1.
-    + inversion H.
-      apply not_interp_interp in E1.
-      rewrite <-H1.
-      assumption.
-    + apply IHl. (*why it works?*)
-      apply H.
-Qed.
-
-
 (*Can't prove! Lemma solver_opt : forall p, find p = find (formula_optimizer p).*)
+
+
+Lemma find_interp: forall p V, find_valuation (formula_optimizer p)=Some V -> interp V p=true.
+Proof.
+  intros.
+  unfold find_valuation in H;
+  unfold try_valuation in H.
+  induction (enum_valuation (collect_var (formula_optimizer p))). (*change here*)
+  - discriminate H. (*valuation list is empty*)
+  - rewrite <-optimizer_correctness in H.
+    destruct (interp a p) eqn: E1.
+    + inversion H. (* interp a p = true => a = V*)
+      rewrite H1 in E1.
+      assumption.
+    + apply IHl. (* interp a p = false*)
+      apply H. (* use hypothesis from induction*)
+Qed.
   
-  
+    
 Lemma solver_sound : forall p, solver p = true -> satisfiable p.
 Proof.
   intros.
-  destruct p;unfold satisfiable;unfold solver in H. 
-  - (*var*)
-    exists (override empty_valuation i true).
-    simpl.
-    unfold override.
-    now rewrite  <- beq_id_refl.
-  - (*bool*)
-    destruct (find_valuation (formula_optimizer (bool b))) eqn:E in H;(try discriminate H).
-    unfold find_valuation in E.  
-    simpl in E.
-    destruct b.    
-    now exists v.
-    discriminate E.
-  -  (*land*)
-    destruct (find_valuation (formula_optimizer(land p1 p2))) eqn:E in H;(try discriminate H).
-    exists v.
-    apply land_interp_interp.
-    apply land_find_interp in E.
+  unfold satisfiable.
+  unfold solver in H.
+  destruct (find_valuation (formula_optimizer p)) eqn:E in H. (*return of find_valuation*) (*change here*)
+  - exists v. (*Some v*)
+    apply find_interp in E.
     assumption.
-  - (*lor*)
-    destruct (find_valuation (formula_optimizer(lor p1 p2))) eqn:E in H;try(discriminate H).
-    exists v.
-    apply lor_interp_interp.
-    apply lor_find_interp in E.
-    assumption.
-  - (* mapsto*)   
-    destruct (find_valuation (formula_optimizer(mapsto p1 p2))) eqn:E in H;try(discriminate H).
-    exists v.
-    apply mapsto_interp_interp.
-    apply mapsto_find_interp in E.
-    assumption.
-  - (* not*)   
-    destruct (find_valuation (formula_optimizer(not p))) eqn:E in H;try(discriminate H).
-    exists v.
-    apply not_interp_interp.
-    apply not_find_interp in E.
-    assumption.
-Qed.      
-                  
-                  
-
-    
-    
-     
-  
+  - discriminate H. (*None*)
+Qed.
