Solver.v
@@ -1,0 +1,73 @@
+Require Import Formula FindVal.
+Require Setoid. 
+
+
+(** Pure SAT solver. *)
+Definition solver (p : form) :bool:=
+  match find_valuation p with
+  | Some _ => true
+  | None => false
+  end.
+
+(** Exercise 2.6*)
+(**
+   Difference between satisfiable and solver.
+   satisfiable is a property of a boolean formula, solver is a method to find out whether a formula is satisfiable. If solver returns true then we can conclude that the formula is satisfiable.
+ **)
+
+Module Test_solver.
+  Definition x := (var (Id "x")).
+  Definition y := (var (Id "y")).
+
+(** Exercise 2.7*)
+  Lemma test_pos_1: solver (land (lor x (not y)) (lor (not x) y) ) =true.
+  Proof.
+    reflexivity.
+  Qed.
+  
+  Lemma test_pos_2: solver (mapsto (not y) (lor x y) ) =true.  
+  Proof.
+    reflexivity.
+  Qed.
+  
+  Lemma test_neg_1: solver (land (land x (not x)) (boolv true)) = false.
+  Proof.
+    reflexivity.
+  Qed.
+  
+  Lemma test_neg_2: solver (land  (not x) (boolv false)) = false.
+  Proof.
+    reflexivity.
+  Qed.
+     
+End Test_solver.
+
+
+Lemma find_interp: forall p V, find_valuation p=Some V -> interp V p=true.
+Proof.
+  intros.
+  unfold find_valuation in H;
+  unfold try_valuation in H.
+  induction (enum_valuation (collect_var p)).
+  - discriminate H. (*valuation list is empty*)
+  - destruct (interp a p) eqn: E1.
+    + inversion H. (* interp a p = true => a = V*)
+      rewrite H1 in E1.
+      assumption.
+    + apply IHl. (* interp a p = false*)
+      apply H. (* use hypothesis from induction*)
+Qed.
+  
+  
+(** Exercise 2.8 *)  
+Lemma solver_sound : forall p, solver p = true -> satisfiable p.
+Proof.
+  intros.
+  unfold satisfiable.
+  unfold solver in H.
+  destruct (find_valuation p) eqn:E in H. (*return of find_valuation*)
+  - exists v. (*Some v*)
+    apply find_interp in E.
+    assumption.
+  - discriminate H. (*None*)
+Qed.
